Checkpoint server proof

src/program_proof/ctrexample/server.v
@@ -3,7 +3,113 @@ From Perennial.goose_lang Require Export ffi.grove_prelude.
 From Perennial.program_proof Require Import proof_prelude.
 From Perennial.goose_lang Require Export ffi.grove_filesys_axioms.
 From Perennial.program_proof.ctrexample Require Import interface.
+From Perennial.program_proof Require Import marshal_proof.
+From Goose.github_com.mit_pdos.gokv.ctrexample Require Import server.
+From Perennial.goose_lang Require Export crash_lock.
+From Perennial.program_proof.ctrexample Require Import wpc_proofmode.
 
 Section server_proof.
+
+Context `{!heapGS Σ}.
+Context `{!filesysG Σ}.
+Context `{!inG Σ mono_natUR}.
+Context `{stagedG Σ}.
+
+Definition ctrname := "ctr".
+
+Definition own_CtrServer_durable (c:u64) : iProp Σ :=
+  ctrname f↦ [] ∗ ⌜c = U64 0⌝ ∨ (∃ l, ctrname f↦ l ∗ ⌜has_encoding l [EncUInt64 c]⌝)
+.
+
+Definition own_CtrServer_ghost γ (c:u64) : iProp Σ :=
+  counter_own γ (int.nat c)
+.
+
+Definition own_CtrServer (s:loc) (c:u64) : iProp Σ :=
+  "Hval" ∷ s ↦[CtrServer :: "val"] #c ∗
+  "Hfilename" ∷ s ↦[CtrServer :: "filename"] #(str ctrname)
+.
+
+Definition ctrServerN := nroot .@ "ctrserver".
+
+Definition is_CtrServer γ (s:loc) : iProp Σ :=
+  ∃ mu,
+  "#Hmu" ∷ readonly (s ↦[CtrServer :: "mu"] mu) ∗
+  "#HmuInv" ∷ is_crash_lock ctrServerN mu
+  (∃ c, own_CtrServer_ghost γ c ∗
+        own_CtrServer_durable c ∗
+        own_CtrServer s c
+  )
+  (∃ c, own_CtrServer_ghost γ c ∗
+        own_CtrServer_durable c)
+.
+
+Lemma wpc_CtrServer__MakeDurable γ (s:loc) c c' {stuck P}:
+  {{{
+       own_CtrServer_ghost γ c ∗ own_CtrServer_durable c ∗ own_CtrServer s c'
+  }}}
+    CtrServer__MakeDurable #s @ stuck ; P
+  {{{
+       RET #(); own_CtrServer_ghost γ c' ∗ own_CtrServer_durable c' ∗ own_CtrServer s c'
+  }}}
+  {{{
+       ∃ c'', own_CtrServer_ghost γ c'' ∗ own_CtrServer_durable c''
+  }}}.
+Proof.
+Admitted.
+
+Lemma wp_CtrServer__FetchAndIncrement γ (s:loc) :
+  {{{
+       is_CtrServer γ s
+  }}}
+    CtrServer__FetchAndIncrement #s
+  {{{
+       (x:u64), RET #x; True
+  }}}
+.
+Proof.
+  iIntros (Φ) "#Hpre HΦ".
+  wp_lam.
+  iNamed "Hpre".
+  wp_loadField.
+  wp_apply (acquire_spec with "HmuInv").
+  { done. }
+  iIntros "Hres".
+  wp_pures.
+  wp_apply wpc_wp.
+  wpc_apply (use_crash_locked with "Hres").
+  { done. }
+  iSplit.
+  { by instantiate (1:=True%I). }
+  iIntros "H".
+  iDestruct "H" as (c) "(Hghost&Hdur&Hvol)".
+
+  iNamed "Hvol".
+  iCache with "Hghost Hdur".
+  {
+    iSplitL ""; first done.
+    iExists c; iFrame.
+  }
+
+  wpc_loadField.
+  wpc_pures.
+  wpc_loadField.
+  wpc_pures.
+  (* FIXME: need no-overflow assumption *)
+  wpc_storeField.
+  wpc_pures.
+  wpc_apply (wpc_CtrServer__MakeDurable with "[$Hghost $Hdur $Hval $Hfilename]").
+  iSplit.
+  { (* crash-condition of MakeDurable ==> our crash condition *)
+    eauto.
+  }
+  iNext.
+  iIntros "(Hghost & Hdur & Hvol)".
+  iCache with "Hghost Hdur".
+  { iSplitL ""; first done. iExists _; iFrame. }
+  wpc_pures.
+  wpc_loadField.
+  (* wpc_apply (release_spec with "[]"). *)
+Admitted.
 
 End server_proof.
