src/program_proof/ctrexample/interface.v
@@ -1,18 +1,18 @@
 From Perennial.goose_lang Require Import prelude.
 From Perennial.goose_lang Require Export ffi.grove_prelude.
 From Perennial.program_proof Require Import proof_prelude.
-From iris.algebra Require Import mono_nat.
+From iris.algebra Require Export mono_nat.
 From Perennial.program_proof.memkv Require Import rpc_spec.
 From Perennial.program_proof Require Import marshal_proof.
 
 Section interface.
 
-Context `{inG Σ mono_natUR}.
-Context `{HPRE: !gooseGlobalGS Σ}.
+Context `{!inG Σ mono_natUR}.
 
 Definition counter_lb γ (x:nat) : iProp Σ := own γ (◯MN x).
 Definition counter_own γ (x:nat) : iProp Σ := own γ (●MN x).
 
+Context `{HPRE: !gooseGlobalGS Σ}.
 Definition FAISpec γ (reqData:list u8) (Φ:list u8 → iProp Σ) : iProp Σ :=
   □(
       ∀ (x:nat), counter_own γ x ={⊤}=∗ counter_own γ (x + 1) ∗
